Prove an additional equiv. corollary, specialized to initial_core.

driver/CompositionalComplements.v
@@ -21,19 +21,8 @@ Unset Printing Implicit Defensive.
 
 Module CE := ContextEquiv LinkingSimulation.
 
-Section CompositionalComplements.
-
 Notation Clight_module := (program Clight.fundef Ctypes.type).
 Notation Asm_module := (AsmEFF.program).
-
-(** [N] is the number of source/target modules. *)
-
-Variable N : pos.
-Variable source_modules : 'I_N -> Clight_module.
-Variable target_modules : 'I_N -> Asm_module.
-Variable plt : ident -> option 'I_N.
-
-(** Wrap the program interaction semantics as module semantics. *)
 
 Definition mk_src_sem (p : Clight_module) :=
   let ge := Genv.globalenv p in 
@@ -43,34 +32,65 @@ Definition mk_tgt_sem (tp : Asm_module) :=
   let tge := Genv.globalenv tp in
   @Modsem.mk AsmEFF.fundef unit tge Asm_coop.state (Asm_eff.Asm_eff_sem hf).
 
+Section CompositionalComplements.
+
+Variable N : pos.
+Variable source_modules : 'I_N -> Clight_module.
+Variable target_modules : 'I_N -> Asm_module.
+Variable plt : ident -> option 'I_N.
+
 Definition sems_S (ix : 'I_N) := mk_src_sem (source_modules ix).
 Definition sems_T (ix : 'I_N) := mk_tgt_sem (target_modules ix).
 
-(** [ge_top] ensures that the globalenvs for the modules agree on the
- set of global blocks. *)
+(** [ge_top] constrains the source--target global envs. of the modules in 
+  sems_S and sems_T to have equal domain. *)
 
 Variable ge_top : ge_ty.
 Variable domeq_S : forall ix : 'I_N, genvs_domain_eq ge_top (sems_S ix).(Modsem.ge).
 Variable domeq_T : forall ix : 'I_N, genvs_domain_eq ge_top (sems_T ix).(Modsem.ge). 
 
-(** The (deterministic) context [C]. [nuke_C] restricts contexts to 
- those that store only valid blocks into memory (this holds of all 
- assembly contexts; see backend/Asm_nucular.v). *)
+(** The target modules are (independently) compiled from source the respective
+  source modules. *)
+
+Variable transf : 
+  forall ix : 'I_N, 
+  transf_clight_program (source_modules ix) 
+  = Errors.OK (target_modules ix).
+
+Lemma find_syms :
+  forall (i : 'I_N) (id : ident) (bf : block),
+  Genv.find_symbol (Modsem.ge (sems_S i)) id = Some bf ->
+  Genv.find_symbol (Modsem.ge (sems_T i)) id = Some bf.
+Proof.
+intros idx id bf.
+unfold sems_S, sems_T; simpl.
+generalize (transf idx); intros H.
+apply transf_clight_program_preserves_syms with (s := id) in H.
+rewrite H; auto.
+Qed.
+
+(** The (deterministic) context [C]. 
+    - [nuke_C] restricts contexts to those that store only valid blocks 
+      (this holds of all assembly contexts; see backend/Asm_nucular.v).
+    - [sim_C]: C self-inject (C <= C).
+  *)
 
 Variable C : Modsem.t.   
 Variable sim_C : 
   SM_simulation.SM_simulation_inject 
-    C.(Modsem.sem) C.(Modsem.sem) C.(Modsem.ge) C.(Modsem.ge).
+  C.(Modsem.sem) C.(Modsem.sem) C.(Modsem.ge) C.(Modsem.ge).
 Variable nuke_C : Nuke_sem.t (Modsem.sem C).
 Variable domeq_C : genvs_domain_eq ge_top C.(Modsem.ge).
 Variable det_C : core_semantics_lemmas.corestep_fun (Modsem.sem C).
 
-(** [NOTE: RC] [CE.linker_S] ensures that both the context [C] the
-  source modules [sems_S] are reach-closed. See file
-  linking/context_equiv.v. *)
+(** [NOTE: RC] [CE.linker_S] ensures that both the context [C] the source
+  modules [sems_S] are reach-closed. See file linking/context_equiv.v for
+  details. *)
 
 Notation source_linked_semantics := (CE.linker_S sems_S plt C).
 Notation target_linked_semantics := (CE.linker_T sems_T plt C).
+Definition safe ge l m := 
+  forall n, closed_safety.safeN source_linked_semantics ge n l m.
 
 Lemma asm_modules_nucular (ix : 'I_N) : Nuke_sem.t (Modsem.sem (sems_T ix)).
 Proof. solve[apply Asm_is_nuc]. Qed.
@@ -80,8 +100,6 @@ Proof. solve[apply Asm_is_nuc]. Qed.
  ensure that each module is well-formed (for example, no module
  defines the same function twice). *)
 
-Variable transf : forall ix : 'I_N, 
-  transf_clight_program (source_modules ix) = Errors.OK (target_modules ix).
 Variable init : forall ix : 'I_N, 
   {m0 | Genv.init_mem (source_modules ix) = Some m0}.
 Variable lnr : forall ix : 'I_N, 
@@ -101,33 +119,42 @@ Qed.
 
 Variable main : Values.val.
 
-Lemma find_syms :
-  forall (i : 'I_N) (id : ident) (bf : block),
-  Genv.find_symbol (Modsem.ge (sems_S i)) id = Some bf ->
-  Genv.find_symbol (Modsem.ge (sems_T i)) id = Some bf.
-Proof.
-intros idx id bf.
-unfold sems_S, sems_T; simpl.
-generalize (transf idx); intros H.
-apply transf_clight_program_preserves_syms with (s := id) in H.
-rewrite H; auto.
-Qed.
-
-Notation lifted_sim := 
-  (CE.lifted_sim asm_modules_nucular plt modules_inject domeq_S domeq_T 
-     find_syms sim_C domeq_C nuke_C main).
-
 (** Starting from matching source--target states, the source/target
  programs equiterminate when linked with [C], assuming the source
  linked program is safe and reach-closed (see [NOTE: RC] above). *)
 
+Notation lifted_sim := 
+  (CE.lifted_sim asm_modules_nucular plt modules_inject domeq_S domeq_T 
+   find_syms sim_C domeq_C nuke_C main).
+
 Theorem context_equiv cd mu l1 m1 l2 m2 
-  (source_safe : forall n, closed_safety.safeN source_linked_semantics ge_top n l1 m1) 
+  (source_safe : safe ge_top l1 m1) 
   (match12 : Wholeprog_sim.match_state lifted_sim cd mu l1 m1 l2 m2) :
   (terminates source_linked_semantics ge_top l1 m1 
    <-> terminates target_linked_semantics ge_top l2 m2).
 Proof. 
 eapply CE.context_equiv; eauto.   
+unfold CE.extend_sems; intros ix; destruct (lt_dec ix N); auto.
+simpl; intros m m' m'' ge c c' c'' H H2. 
+simpl in H, H2; eapply asm_step_det; eauto.
+Qed.
+
+(** The following corollary (really, of CE.context_equiv) specializes
+  to entry point main. *)
+
+Theorem init_context_equiv l1 m1 m2 j vals1 vals2
+  (source_safe : safe ge_top l1 m1)
+  (init1 : initial_core source_linked_semantics ge_top main vals1 = Some l1)
+  (init1_inv : cc_init_inv j ge_top vals1 m1 ge_top vals2 m2) :
+  exists l2, 
+  [/\ initial_core target_linked_semantics ge_top main vals2 = Some l2
+    & (terminates source_linked_semantics ge_top l1 m1 
+   <-> terminates target_linked_semantics ge_top l2 m2)].
+Proof. 
+eapply CE.init_context_equiv; eauto.
+apply: asm_modules_nucular.
+apply: modules_inject.
+apply: find_syms.
 unfold CE.extend_sems; intros ix; destruct (lt_dec ix N); auto.
 simpl; intros m m' m'' ge c c' c'' H H2. 
 simpl in H, H2; eapply asm_step_det; eauto.
